\documentclass[notes]{subfiles}

\begin{document}

\setcounter{section}{19}
\section{Lecture (4/9/25)}

\subsection{Laplace Transform Theorems}
Evaluating the laplace transform of functions like $e^t t^2 \sin(3t)$ can be difficult. Therefore, it would be nice if we could break this down into its product components.

\begin{theorem}[First Laplace Translation Theorem] \label{first_translation_theorem}
    If $f$ is a function of exponential type and $a \in \real$ then
    \[
        \lap(e^{at}f(t)) = (\lap f)(s - a)
    \]
\end{theorem}
\begin{proof}
    \begin{align*}
        \lap(e^{at}f(t))
        &= \int_0^\infty e^{at}f(t)e^{-st}dt
        = \int_0^\infty f(t)e^{-(s - a)t}dt
        = (\lap f)(s - a)
    \end{align*}
\end{proof}

\begin{exercise}
    Calculate $\lap(t^3e^{5t})$.
\end{exercise}
\begin{solution}
    \begin{align*}
        \lap(t^3e^{5t})
        &= \frac{3!}{s^4}\Big|_{s = s - 5}
        = \frac{3!}{(s - 5)^4}
    \end{align*}
\end{solution}

\begin{exercise}
    Calculate $\lap(e^{-2t}\cos(4t))$.
\end{exercise}
\begin{solution}
    \begin{align*}
        \lap(e^{-2t}\cos(4t))
        &= \frac{s}{s^2 + 16}\Big|_{s = s + 2}
        = \frac{s + 2}{(s + 2)^2 + 16}
    \end{align*}
\end{solution}

\begin{exercise} \label{useful_inv_laplace_transform}
    Calculate $\lap^{-1} \left(\frac{2s + 5}{(s - 3)^2} \right)$.
\end{exercise}
\begin{solution}
    \begin{align*}
        \lap^{-1} \left(\frac{2s + 5}{(s - 3)^2} \right)
        &= \lap^{-1} \left( \frac{A}{s - 3} + \frac{B}{(s - 3)^2} \right)
        = Ae^{3t} + Bt e^{3t}
    \end{align*}
    So
    \begin{align*}
        &2s + 5 = A(s - 3) + B \\
        s = 3 \implies& 6 + 5 = B \iff B = 11 \\
        s = 4 \implies& 8 + 5 = A + 11 \iff 13 = A + 11 \iff A = 2
    \end{align*}
    Therefore
    \begin{align*}
        \lap^{-1} \left(\frac{2s + 5}{(s - 3)^2} \right)
        &= 2e^{3t} + 11t e^{3t}
    \end{align*}
\end{solution}

\begin{exercise}
    Calculate $\lap^{-1} \left( \frac{\frac{s}{2} + \frac{5}{3}}{s^2 + 4s + 6} \right)$.
\end{exercise}
\begin{solution}
    \begin{align*}
        \lap^{-1} \left( \frac{\frac{s}{2} + \frac{5}{3}}{s^2 + 4s + 6} \right)
        &= \lap^{-1} \left( \frac{\frac{s}{2} + \frac{5}{3}}{s^2 + 4s + 4 + 6 - 4} \right)
        = \lap^{-1} \left( \frac{\frac{s}{2} + \frac{5}{3}}{(s + 2)^2 + 2} \right) \\
        &= \lap^{-1} \left( \frac{1}{2}\left(\frac{s}{(s + 2)^2 + 2}\right) + \frac{\frac{5}{3}}{(s + 2)^2 + 2} \right) \\
        &= \lap^{-1} \left( \frac{1}{2}\left(\frac{s + 2 - 2}{(s + 2)^2 + 2}\right) + \frac{\frac{5}{3}}{(s + 2)^2 + 2} \right) \\
        &= \lap^{-1} \left( \frac{1}{2}\left(\frac{s + 2}{(s + 2)^2 + 2}\right) + \frac{\frac{5}{3} - 1}{(s + 2)^2 + 2} \right) \\
        &= \frac{1}{2}e^{-2t}\cos(\sqrt{2}t) + \frac{2}{3}\lap^{-1} \left( \frac{1}{(s + 2)^2 + 2} \right) \\
        &= \frac{1}{2}e^{-2t}\cos(\sqrt{2}t) + \frac{\sqrt{2}}{3}\lap^{-1} \left( \frac{\sqrt{2}}{(s + 2)^2 + 2} \right) \\
        &= \frac{1}{2}e^{-2t}\cos(\sqrt{2}t) + \frac{\sqrt{2}}{3}e^{-2t}\sin(\sqrt{2}t)
    \end{align*}
\end{solution}

\begin{exercise}
    Solve $y'' - 6y' + 9y = t^2 e^{3t}$ with initial conditions at $t = 0$ of $y = 2$ and $y' = 17$.
\end{exercise}
\begin{solution}
    \begin{align*}
        &y'' - 6y' + 9y = t^2 e^{3t} \\
        \iff& s^2 Y - sy|_{t = 0} - y'|_{t = 0} - 6(sY - y|_{t = 0}) + 9Y = \frac{2!}{s^3}\Big|_{s = s - 3} \\
        \iff& s^2 Y - 2s - 17 - 6(sY - 2) + 9Y = \frac{2}{(s - 3)^3} \\
        \iff& Y(s^2 - 6s + 9) = \frac{2}{(s - 3)^3} + 2s + 17 - 12 = \frac{2}{(s - 3)^3} + 2s + 5 \\
        \iff& Y(s - 3)^2 = \frac{2}{(s - 3)^3} + 2s + 5 \\
        \iff& Y = \frac{2}{(s - 3)^5} + \frac{2s + 5}{(s - 3)^2} = \frac{2}{4!}\left(\frac{4!}{(s - 3)^5}\right) + \frac{2s + 5}{(s - 3)^2} = \frac{1}{12}\left(\frac{4!}{(s - 3)^5}\right) + \frac{2s + 5}{(s - 3)^2} \\
        \iff& y = \frac{1}{12}t^4 e^{3t} + 2e^{3t} + 11t e^{3t} \qquad \text{By \cref{useful_inv_laplace_transform}}
    \end{align*}
\end{solution}

We saw in \cref{first_translation_theorem} how a change in the $t$-domain shifted the $s$-domain. We will now show that a change in the $s$-domain will shift the $t$-domain.
\begin{theorem}[Second Laplace Translation Theorem]
    If $f$ is a function such that \\ $t \mapsto f(t - a)\heav(t - a)$ is of exponential form and $a \in \real$ then
    \[
        \lap(f(t - a)\heav(t - a)) = e^{-as}\lap f(s)
    \]
\end{theorem}
\begin{proof}
    \begin{align*}
        \lap(f(t - a)\heav(t - a))
        &= \int_0^\infty f(t - a)\heav(t - a)e^{-st}dt
        = \int_a^\infty f(t - a)e^{-st}dt \\
        &= \lim_{b\to\infty} \int_a^b f(t - a)e^{-st}dt
    \end{align*}
    Let $u = t - a \iff t = u + a \implies du = dt$
    \begin{align*}
        \lap(f(t - a)\heav(t - a))
        &= \lim_{b\to\infty} \int_a^b f(t - a)e^{-st}dt
        = \lim_{b\to\infty} \int_0^{b - a} f(u)e^{-s(u + a)}du \\
        &= \int_0^\infty f(u)e^{-su}e^{-as}du
        = e^{-as}\int_0^\infty f(u)e^{-su}du
        = e^{-as}\int_0^\infty f(t)e^{-st}dt \\
        &= e^{-as}\lap f(s)
    \end{align*}
\end{proof}

\begin{exercise}
    Find the Laplace transform of $2 - 3\heav(t - 2) + \heav(t - 3)$.
\end{exercise}
\begin{solution}
    \begin{align*}
        \lap(2 - 3\heav(t - 2) + \heav(t - 3))
        &= \frac{2}{s} - \frac{3e^{-2s}}{s} - \frac{e^{-3s}}{s}
        = \frac{2 - 3e^{-2s} - e^{-3s}}{s}
    \end{align*}
\end{solution}

\begin{exercise}
    Calculate $\lap^{-1} \left( \frac{e^{-2s}}{s - 4} \right)$.
\end{exercise}
\begin{solution}
    \begin{align*}
        \lap^{-1} \left( \frac{e^{-2s}}{s - 4} \right)
        &= e^{4t}\heav(t)|_{t = t - 2}
        = e^{4(t - 2)}\heav(t - 2)
    \end{align*}
\end{solution}

\begin{exercise}
    Calculate $\lap^{-1} \left( \frac{se^{-\frac{\pi}{2}s}}{s^2 + 9} \right)$.
\end{exercise}
\begin{solution}
    \begin{align*}
        \lap^{-1} \left( \frac{se^{-\frac{\pi}{2}s}}{s^2 + 9} \right)
        &= \cos(3t)\heav(t)|_{t = t - \frac{\pi}{2}}
        = \cos\left(3\left(t - \frac{\pi}{2}\right)\right)\heav\left(t - \frac{\pi}{2}\right)
    \end{align*}
\end{solution}

\begin{exercise}
    Solve the IVP $y' + y = f(t)$ where $y|_{t = 0} = 5$ and
    \[
        f(t) = \begin{cases}
            0 & 0 \leq t < \pi \\
            3\cos t & t \geq \pi
        \end{cases}
    \]
\end{exercise}
\begin{solution}
    First consider that
    \begin{align*}
        f(t)
        &= 3\cos(t)\heav(t - \pi)
        = -3\cos(t - \pi)\heav(t - \pi)
    \end{align*}
    Now we can consider that
    \begin{align*}
        &y' + y = -3\cos(t - \pi)\heav(t - \pi)
        \iff sY - y|_{t = 0} + Y = 3e^{-\pi s}\left(\frac{s}{s^2 + 1}\right) \\
        \iff& Y(s + 1) = 3e^{-\pi s}\left(\frac{s}{s^2 + 1}\right) + 5
        \iff Y = 3e^{-\pi s}\left(\frac{s}{(s^2 + 1)(s + 1)}\right) + \frac{5}{s + 1} \\
        \iff& y = \lap^{-1} \left( 3e^{-\pi s}\left(\frac{s}{(s^2 + 1)(s + 1)}\right) + \frac{5}{s + 1} \right)
    \end{align*}
    Now we consider that
    \begin{align*}
        y
        &= \lap^{-1} \left( 3e^{-\pi s}\left(\frac{s}{(s^2 + 1)(s + 1)}\right) + \frac{5}{s + 1} \right)
        = 3 \lap^{-1} \left(e^{-\pi s}\left(\frac{s}{(s^2 + 1)(s + 1)}\right)\right) + 5e^{-t} \\
        &= 3 \lap^{-1} \left(e^{-\pi s}\left(\frac{As + B}{s^2 + 1} + \frac{C}{s + 1}\right)\right) + 5e^{-t} \\
        &= 3 \lap^{-1} \left(e^{-\pi s}\left(\frac{As}{s^2 + 1} + \frac{B}{s^2 + 1} + \frac{C}{s + 1}\right)\right) + 5e^{-t} \\
        &= 3\heav(t)(A\cos t + B\sin t + Ce^{-t})|_{t = t - \pi} + 5e^{-t} \\
        &= 3\heav(t - \pi)(A\cos(t - \pi) + B\sin(t - \pi) + Ce^{-(t - \pi)}) + 5e^{-t}
    \end{align*}
    Therefore
    \begin{align*}
        &s = (As + B)(s + 1) + C(s^2 + 1) \\
        s = i \implies& i = (iA + B)(i + 1) = -A + iA + iB + B = (-A + B) + i(A + B) \\
        \iff& 0 = -A + B \iff A = B \\
        \iff& 1 = A + B = 2A \iff A = B = \frac{1}{2} \\
        s = -1 \implies& -1 = 2C \iff C = -\frac{1}{2}
    \end{align*}
    So our solution is
    \[
        y = \frac{3}{2}\heav(t - \pi)(\cos(t - \pi) + \sin(t - \pi) - e^{-(t - \pi)}) + 5e^{-t}
    \]
\end{solution}

\end{document}