\documentclass[notes]{subfiles}
\externaldocument{lecture_11}

\begin{document}

\setcounter{section}{17}
\section{Lecture (4/7/25)}

\subsection{Laplace Transform of Derivatives}
\begin{theorem}
    If $f$ is a $C^n$ function of exponential type then
    \[
        \mathcal{L}D^n f(s) = s^n(\mathcal{L}f(s)) - \sum_{i = 1}^n s^{n - i}(D^{i - 1}f(0))
    \]
    for $s \geq 0$
\end{theorem}
\begin{proof}
    For the base case of $n = 0$ consider that
    \begin{align*}
        s^0(\mathcal{L}f(s)) - \sum_{i = 1}^0 s^{n - i}(D^{i - 1}f(0))
        &= \mathcal{L}f(s)
    \end{align*}
    We now assume our induction hypothesis and consider
    \begin{align*}
        \mathcal{L}D^{n + 1} f(s)
        &= \int_0^\infty (D^{n + 1}f(s))e^{-st}dt
        = \lim_{b\to\infty} \int_0^b (D^{n + 1}f(s))e^{-st}dt
    \end{align*}
    Let $u = e^{-st} \implies du = -se^{-st}dt$ and $dv = D^{n + 1}f(s)dt \impliedby v = D^n f(s)$ so
    \begin{align*}
        (\mathcal{L}D^{n + 1} f)(s)
        &= \int_0^\infty (D^{n + 1}f(s))e^{-st}dt
        = \lim_{b\to\infty} \left( D^n f(s)e^{-st}\Big|_{t = 0}^{t = b} + s\int_0^b (D^n f(s))e^{-st}dt \right) \\
        &= \lim_{b\to\infty} (D^n f(b)e^{-sb} - D^n f(0)) + s\int_0^\infty (D^n f(s))e^{-st}dt \\
        &= -D^n f(0) + s(\mathcal{L}D^n f(s))
        = s(\mathcal{L}D^n f(s)) - D^n f(0)
    \end{align*}
    Then by our induction hypothesis
    \begin{align*}
        (\mathcal{L}D^{n + 1} f)(s)
        &= s(\mathcal{L}D^n f(s)) - D^n f(0) \\
        &= s(s^n(\mathcal{L}f(s)) - \sum_{i = 1}^n s^{n - i}(D^{i - 1}f(0))) - D^n f(0) \\
        &= s^{n + 1}(\mathcal{L}f(s)) - \sum_{i = 1}^n s^{(n + 1) - i}(D^{i - 1}f(0)) - s^0 (D^n f(0)) \\
        &= s^{n + 1}(\mathcal{L}f(s)) - \sum_{i = 1}^n s^{(n + 1) - i}(D^{i - 1}f(0)) - \sum_{i = n + 1}^{n + 1} s^{(n + 1) - i}(D^{i - 1}f(0)) \\
        &= s^{n + 1}(\mathcal{L}f(s)) - \sum_{i = 1}^{n + 1} s^{(n + 1) - i}(D^{i - 1}f(0))
    \end{align*}
\end{proof}

\begin{corollary}
    If $f$ is a $C^1$ function of exponential type then
    \[
        \mathcal{L}f'(s) = s(\mathcal{L}f(s)) - f(0)
    \]
    for $s \geq 0$
\end{corollary}

\begin{corollary}
    If $f$ is a $C^2$ function of exponential type then
    \[
        \mathcal{L}f''(s) = s^2(\mathcal{L}f(s)) - sf(0) - f'(0)
    \]
    for $s \geq 0$
\end{corollary}



\end{document}