\documentclass[notes]{subfiles}

\begin{document}

\setcounter{section}{9}
\section{Lecture (2/19/25)}
\subsection{Reduction of Order}
The idea here is that if we are given an order two homogeneous linear ODE, a basis solution $y_1$, then we can find the basis solution $y_2$ such that the general solution is $y = c_1y_1 + c_2y_2$.

We are given an order two homogeneous linear ODE in the form
\[
    a_2(x)y'' + a_1(x)y' + a_0(x)y = 0
\]
such that $a_2(x) \neq 0$ for all $x \in I$. We are given $y_1$ as a basis solution.

We will now rewrite as
\begin{align*}
    a_2(x)y'' + a_1(x)y' + a_0(x)y = 0
    &\iff y'' + \frac{a_1(x)}{a_2(x)}y' + \frac{a_0(x)}{a_2(x)}y = 0 \\
    &\iff y'' + P(x)y' + Q(x)y = 0
\end{align*}
Now the trick here is to let $y_2 = uy_1$ therefore
\begin{align*}
    y_2 = uy_1
    &\iff y_2' = u'y_1 + uy_1' \\
    &\iff y_2'' = u''y_1 + u'y_1' + u'y_1' + uy_1'' = u''y_1 + 2u'y_1' + uy_1'' % haha you are a binomial
\end{align*}

Now we plug $y_2$ in as a solution so

\begin{align*}
    0
    &= y_2'' + P(x)y_2' + Q(x)y_2 \\
    &= (u''y_1 + 2u'y_1' + uy_1'') + P(x)(u'y_1 + uy_1') + Q(x)(uy_1) \\
    &= u(y_1'' + P(x)y_1' + y_1) + u''y_1 + 2u'y_1' + P(x)(u'y_1) \\
    &= u''y_1 + 2u'y_1' + P(x)(u'y_1) \\
    &= y_1u'' + (2y_1' + P(x)y_1)u'
\end{align*}

To get this in the form of a linear ODE we make the substitution $w = u'$ solution

\begin{align*}
    y_1w' + (2y_1' + P(x)y_1)w = 0
    &\iff y_1\frac{dw}{dx} = -(2y_1' + P(x)y_1)w \\
    &\iff y_1dw = -(2y_1' + P(x)y_1)wdx \\
    &\iff \frac{1}{w}dw = -\frac{2y_1' + P(x)y_1}{y_1}dx = \left( -\frac{2y_1'}{y_1} - P(x) \right)dx \\
    &\iff \int \frac{1}{w}dw = -\int \frac{2y_1'}{y_1}dx - \int P(x)dx \\
    &\iff \ln(w) = -2\ln(y_1) - \int P(x)dx \\
    &\iff w = e^{-2\ln(y_1)}e^{-\int P(x)dx} = \frac{e^{-\int P(x)dx}}{y_1^2} \\
    &\iff u = \int \frac{e^{-\int P(x)dx}}{y_1^2} dx
\end{align*}

Therefore we can now express $y_2$ as
\[
    y_2 = y_1\int \frac{e^{-\int P(x)dx}}{y_1^2} dx
\]
This formula should be memorized.



\end{document}