\documentclass[notes]{subfiles}

\begin{document}

\setcounter{section}{12}
\section{Lecture (3/3/25)}

\subsection{Annihilation Procedure}
\begin{procedure}[Solving by annihilation]
    ~

    \begin{enumerate}[label = (\arabic*)]
        \item Solve for the basis solutions
        \item Write in operator form
        \item Find annihilator for driver
        \item Apply annihilator
        \item Solve homogeneous ODE
        \item Pick out new solutions
        \item Find constants for particular solution
    \end{enumerate}
\end{procedure}

\begin{exercise}
    Solve $y'' + y = x\cos x - \cos x$ by annihilation.
\end{exercise}
\begin{solution}
    Consider the characteristic polynomial of the associated homogeneous ODE so
    \begin{align*}
        0 = m^2 + 1 = (m - i)(m + 1)
        &\iff m = \pm i
    \end{align*}
    Therefore $y_n = c_1 \cos x + c_2 \sin x$. If we weren't solving by annihilation we could consider $y_p = (Ax + B)\cos x$ but then it would be linearly dependent with the basis solutions. So we would guess $y_p = (Ax^2 + Bx)\cos x$.
    
    For solving by annihilation, let $g(x) = x\cos x - \cos x$ so the operator form is $D^2 + 1 = g$.

    Notice that $D^2 + 1$ annihilates just the second term of $g$. By reduction of order, we can simply bump the multiplicity up to get $(D^2 + 1)^2$ as an annihilator for $g$, therefore
    \begin{align*}
        D^2 + 1 = g
        &\iff (D^2 + 1)^2(D^2 + 1) = (D^2 + 1)^2 g \\
        &\iff (D^2 + 1)^3 = 0
    \end{align*}
    Therefore we can consider the characteristic polynomial so
    \begin{align*}
        0 = (m^2 + 1)^3 = (m - i)^3(m + i)^3
        &\iff m = \pm i
    \end{align*}
    Therefore since we have multiplicity $3$ then the solution to the annihilated ODE is
    \[
        y = c_1\cos x + c_2\sin x + c_3x\cos x + c_4x\sin x + c_5x^2\cos x + c_6x^2\sin x
    \]
    Since we have gained $4$ new terms then the particular solution must be
    \[
        y_p = c_3x\cos x + c_4x\sin x + c_5x^2\cos x + c_6x^2\sin x
    \]
    Relabelling and factoring we get the same as the guess so
    \[
        y_p = (Ax^2 + Bx)\cos x + (Cx^2 + Dx)\sin x
    \]
    Now we find derivatives
    \begin{align*}
        y_p'
        &= (2Ax + B)\cos x - (Ax^2 + Bx)\sin x + (2Cx + D)\sin x + (Cx^2 + Dx)\cos x \\
        &= (Cx^2 + (2A + D)x + B)\cos x + (-Ax^2 + (-B + 2C)x + D)\sin x
    \end{align*}
    and
    \begin{align*}
        y_p''
        &= (2Cx + 2A + D)\cos x - (Cx^2 + (2A + D)x + B)\sin x \\ &+ (-2Ax - B + 2C)\sin x + (-Ax^2 + (-B + 2C)x + D)\cos x \\
        &= (-Ax^2 + (-B + 4C)x + 2A + 2D)\cos x + (-Cx^2 + (-4A - D)x - 2B + 2C)\sin x
    \end{align*}
    And build the ODE
    \begin{align*}
        x\cos x - \cos x
        &= (-Ax^2 + (-B + 4C)x + 2A + 2D)\cos x \\
        &+ (-Cx^2 + (-4A - D)x - 2B + 2C)\sin x \\
        &+ (Ax^2 + Bx)\cos x + (Cx^2 + Dx)\sin x \\
        &= (4Cx + 2A + 2D)\cos x + (-4Ax - 2B + 2C)\sin x
    \end{align*}
    iff
    \begin{align*}
        &(4Cx + 2A + 2D)\cos x + (-4Ax - 2B + 2C)\sin x = (x - 1)(\cos x) \\
        \iff& 4C = 1 \iff C = \frac{1}{4} \\
        \iff& -4A = 0 \iff A = 0 \\
        \iff& 2A + 2D = -1 \iff 2D = -1 \iff D = -\frac{1}{2} \\
        \iff& -2B + 2C = 0 \iff B = C = \frac{1}{4}
    \end{align*}
    So the particular solution is $y_p = \frac{1}{4}x\cos x + \left( \frac{1}{4}x^2 - \frac{1}{2}x \right)\sin x$. Therefore
    \[
        y = c_1 \cos x + c_2 \sin x + \frac{1}{4}x\cos x + \left( \frac{1}{4}x^2 - \frac{1}{2}x \right)\sin x
    \]
    solves the ODE.
\end{solution}

\end{document}